42.v
@@ -90,6 +90,9 @@ End Ex2.
 (* Ex. 3 *)
 Module Ex3.
 
+Require Import List.
+Import ListNotations.
+
 Require Import Bool.
 
 Definition var : Set := nat.
@@ -151,11 +154,6 @@ Proof.
       | |- context [negb ?b] => destruct b; cbn
       | |- context [?b1 || ?b2] => destruct b1, b2
   end; auto.
-(*Restart.
-  induction f; cbn; intros; auto.
-    try f_equal; auto.
-    try f_equal; auto.
-    try f_equal; auto.*)
 Qed.
 
 Inductive nnf_prop : Set :=
@@ -204,188 +202,7 @@ Proof.
   rewrite ?nnf_negate_correct; f_equal; auto.
 Qed.
 
-Inductive literal : Set :=
-    | pos : var -> literal
-    | neg : var -> literal.
-
-Function distr_or (p : nnf_prop) : nnf_prop :=
-match p with
-    | nnf_var v => nnf_var v
-    | nnf_not v => nnf_not v
-    | nnf_and p1 p2 => nnf_and (distr_or p1) (distr_or p2)
-    | nnf_or p1 p2 =>
-        match distr_or p1, distr_or p2 with
-            | nnf_and p1_1 p1_2, p2' =>
-                nnf_and (nnf_or p1_1 p2') (nnf_or p1_2 p2')
-            | p1', nnf_and p2_1 p2_2 =>
-                nnf_and (nnf_or p1' p2_1) (nnf_or p1' p2_2)
-            | p1', p2' => nnf_or p1' p2'
-        end
-end.
-
-Lemma distr_or_correct :
-  forall (truth : var -> bool) (p : nnf_prop),
-    ndenote truth (distr_or p) = ndenote truth p.
-Proof.
-  intros. functional induction distr_or p; cbn;
-  rewrite ?IHn ?IHn0; auto; repeat 
-  match goal with
-      | H : ?a = _, H' : ndenote _ ?a = _ |- _ => rewrite H in H'; cbn in H'
-      | |- context [?b1 || ?b2] => destruct b1, b2; cbn in *
-  end; auto.
-Qed.
-
-Function distr_and (p : nnf_prop) : nnf_prop :=
-match p with
-    | nnf_var v => nnf_var v
-    | nnf_not v => nnf_not v
-    | nnf_and p1 p2 =>
-        match distr_and p1, distr_and p2 with
-            | nnf_or p1_1 p1_2, p2' =>
-                nnf_or (nnf_and p1_1 p2') (nnf_and p1_2 p2')
-            | p1', nnf_or p2_1 p2_2 =>
-                nnf_or (nnf_and p1' p2_1) (nnf_and p1' p2_2)
-            | p1', p2' => nnf_and p1' p2'
-        end
-    | nnf_or p1 p2 => nnf_or (distr_and p1) (distr_and p2)
-end.
-
-Lemma distr_and_correct :
-  forall (truth : var -> bool) (p : nnf_prop),
-    ndenote truth (distr_and p) = ndenote truth p.
-Proof.
-  intros. functional induction distr_and p; cbn;
-  rewrite ?IHn ?IHn0; auto; repeat 
-  match goal with
-      | H : ?a = _, H' : ndenote _ ?a = _ |- _ => rewrite H in H'; cbn in H'
-      | |- context [?b1 && ?b2] => destruct b1, b2; cbn in *
-  end; auto.
-Qed.
-
-(*Definition s := f_and (f_var 1) (f_var 2).*)
-
-Definition cnf (f : formula) : nnf_prop :=
-  distr_or (push_not (unarrow f)).
-
-Lemma cnf_correct :
-  forall (truth : var -> bool) (f : formula),
-    ndenote truth (cnf f) = fdenote truth f.
-Proof.
-  intros. unfold cnf.
-  by rewrite distr_or_correct push_not_correct unarrow_correct.
-Qed.
-
-Definition empty : var -> bool := fun _ => false.
-
-Definition satisfiable (p : prop) : Prop :=
-  exists truth : var -> bool, pdenote truth p = true.
-
-Lemma satisfiable_pvar :
-  forall (v : var) (truth : var -> bool),
-    truth v = true -> satisfiable (pvar v).
-Proof.
-  red. eauto.
-Qed.
-
-Lemma satisfiable_pnot :
-  forall p : prop, (forall truth : var -> bool, pdenote truth p = false) ->
-    satisfiable (pnot p).
-Proof.
-  destruct p; red; cbn; intro; exists (fun _ => false); by rewrite ?H.
-Qed.
-
-(*Lemma satisfiable_pand :
-  forall (p1 p2 : prop) (truth : var -> bool),
-    satisfiable p1 -> satisfiable truth p2 -> satisfiable (pand p1 p2).
-Proof.*)
-
-Lemma safisfiable_por :
-  forall p1 p2 : prop,
-    satisfiable p1 \/ satisfiable p2 -> satisfiable (por p1 p2).
-Proof.
-  unfold satisfiable. intros. decompose [or ex] H;
-  cbn; exists x.
-    by rewrite H1.
-    by rewrite orb_comm H1.
-Qed.
-
-Definition cnf_clause := list literal.
-Definition dnf_clause := list literal.
-
-Require Import List.
-Import ListNotations.
-
-Definition ldenote (truth : var -> bool) (l : literal) : bool :=
-match l with
-    | pos v => truth v
-    | neg v => negb (truth v)
-end.
-
-Fixpoint ccdenote (truth : var -> bool) (cc : cnf_clause) : bool :=
-match cc with
-    | [] => false
-    | h :: t => ldenote truth h || ccdenote truth t
-end.
-
-Lemma ccdenote_app :
-  forall (truth : var -> bool) (c1 c2 : cnf_clause),
-    ccdenote truth (c1 ++ c2) = ccdenote truth c1 || ccdenote truth c2.
-Proof.
-  induction c1; cbn; intro; by rewrite // IHc1 orb_assoc.
-Qed.
-
-Fixpoint dcdenote (truth : var -> bool) (cc : cnf_clause) : bool :=
-match cc with
-    | [] => false
-    | h :: t => ldenote truth h && ccdenote truth t
-end.
-
-Definition cnf_prop : Set := list cnf_clause.
-Definition dnf_prop : Set := list dnf_clause.
-
-Fixpoint cdenote (truth : var -> bool) (p : cnf_prop) : bool :=
-match p with
-    | [] => true
-    | h :: t => ccdenote truth h && cdenote truth t
-end.
-
-Lemma cdenote_app :
-  forall (truth : var -> bool) (p1 p2 : cnf_prop),
-    cdenote truth (p1 ++ p2) = cdenote truth p1 && cdenote truth p2.
-Proof.
-  induction p1; cbn; intro; by rewrite // IHp1 andb_assoc.
-Qed.
-
-Fixpoint ddenote (truth : var -> bool) (p : cnf_prop) : bool :=
-match p with
-    | [] => false
-    | h :: t => dcdenote truth h || ddenote truth t
-end.
-
-Fixpoint toCNF (p : nnf_prop) : cnf_prop :=
-match p with
-    | nnf_var v => [[pos v]]
-    | nnf_not v => [[neg v]]
-    | nnf_and p1 p2 => toCNF p1 ++ toCNF p2
-    | nnf_or p1 p2 => [concat (toCNF p1 ++ toCNF p2)]
-end.
-
-Lemma toCNF_correct :
-  forall (truth : var -> bool) (p : nnf_prop),
-    cdenote truth (toCNF p) = ndenote truth p.
-Proof.
-  induction p; cbn.
-    by rewrite orb_false_r andb_true_r.
-    by rewrite orb_false_r andb_true_r.
-    by rewrite cdenote_app IHp1 IHp2.
-    rewrite concat_app ccdenote_app.
-Abort.
-
-Goal forall (truth : var -> bool) (p : cnf_prop),
-  cdenote truth p = ccdenote truth (concat p).
-Proof.
-  induction p; cbn.
-Abort.
+(* Nonempty lists *)
 
 Inductive nel (A : Type) : Type :=
     | singl : A -> nel A
@@ -394,36 +211,235 @@ Inductive nel (A : Type) : Type :=
 Arguments singl [A].
 Arguments ncons [A] _ _.
 
-Function toCNF' (p : nnf_prop) : cnf_prop :=
-match p with
-    | nnf_var v => [[pos v]]
-    | nnf_not v => [[neg v]]
-    | nnf_and p1 p2 => toCNF' p1 ++ toCNF' p2
-    | nnf_or p1 p2 =>
-        match toCNF' p1, toCNF' p2 with
-            | nnf_and p1_1 p1_2, p2' =>
-                nnf_and (nnf_or p1_1 p2') (nnf_or p1_2 p2')
-            | p1', nnf_and p2_1 p2_2 =>
-                nnf_and (nnf_or p1' p2_1) (nnf_or p1' p2_2)
-            | p1', p2' => concat (p1' ++ p2')
-        end
+Fixpoint nel_app {A : Type} (l1 l2 : nel A) : nel A :=
+match l1 with
+    | singl x => ncons x l2
+    | ncons h t => ncons h (nel_app t l2)
 end.
 
-Fixpoint toDNF (p : nnf_prop) : dnf_prop :=
-match p with
-    | nnf_var v => [[pos v]]
-    | nnf_not v => [[neg v]]
-    | nnf_and p1 p2 => [concat (toDNF p1 ++ toDNF p2)]
-    | nnf_or p1 p2 => toDNF p1 ++ toDNF p2
+Notation "l1 +++ l2" := (nel_app l1 l2) (at level 40). 
+
+Fixpoint nel_bind {A B : Type} (l : nel A) (f : A -> nel B)
+  : nel B :=
+match l with
+    | singl x => f x
+    | ncons h t => f h +++ nel_bind t f
 end.
 
-Definition dnf (f : formula) : nnf_prop :=
+Definition nel_prod {A : Type} (l1 l2 : nel (nel A)) : nel (nel A) :=
+  nel_bind l1 (fun x =>
+    nel_bind l2 (fun y => singl (x +++ y))).
+
+(* Literals *)
+Inductive literal : Set :=
+    | pos : var -> literal
+    | neg : var -> literal.
+
+Definition ldenote (truth : var -> bool) (l : literal) : bool :=
+match l with
+    | pos v => truth v
+    | neg v => negb (truth v)
+end.
+
+Definition clause := nel literal.
+
+(* CNF translation *)
+
+Fixpoint ccdenote (truth : var -> bool) (cc : clause) : bool :=
+match cc with
+    | singl x => ldenote truth x
+    | ncons h t => ldenote truth h || ccdenote truth t
+end.
+
+Lemma ccdenote_app :
+  forall (truth : var -> bool) (c1 c2 : clause),
+    ccdenote truth (c1 +++ c2) = ccdenote truth c1 || ccdenote truth c2.
+Proof.
+  induction c1; cbn; intro; by rewrite // IHc1 orb_assoc.
+Qed.
+
+Definition cnf_prop : Set := nel clause.
+
+Fixpoint cdenote (truth : var -> bool) (p : cnf_prop) : bool :=
+match p with
+    | singl c => ccdenote truth c
+    | ncons h t => ccdenote truth h && cdenote truth t
+end.
+
+Lemma cdenote_app :
+  forall (truth : var -> bool) (p1 p2 : cnf_prop),
+    cdenote truth (p1 +++ p2) = cdenote truth p1 && cdenote truth p2.
+Proof.
+  induction p1; cbn; intro; by rewrite // IHp1 andb_assoc.
+Qed.
+
+Lemma cdenote_bind_l :
+  forall (p : cnf_prop) (truth : var -> bool) (c : clause),
+    cdenote truth (nel_bind p (fun x : nel literal => singl (x +++ c))) =
+    cdenote truth p || ccdenote truth c.
+Proof.
+  induction p; cbn; intros;
+  by rewrite ccdenote_app // IHp -orb_andb_distrib_l.
+Qed.
+
+Lemma cdenote_bind_r :
+  forall (p : cnf_prop) (truth : var -> bool) (c : clause),
+    cdenote truth (nel_bind p (fun x : nel literal => singl (c +++ x))) =
+    cdenote truth p || ccdenote truth c.
+Proof.
+  induction p; cbn; intros;
+  by rewrite ccdenote_app orb_comm // IHp -orb_andb_distrib_l.
+Qed.
+
+Ltac solve_bool := repeat (rewrite -?orb_assoc -?andb_assoc;
+match goal with
+    | |- context [?b1 || ?b2] => destruct b1; cbn; rewrite ?orb_true_l
+    | |- context [?b1 && ?b2] => destruct b1; cbn; rewrite ?andb_false_l
+end; auto).
+
+Lemma cdenote_nel_prod :
+  forall (truth : var -> bool) (p1 p2 : cnf_prop),
+    cdenote truth (nel_prod p1 p2) = cdenote truth p1 || cdenote truth p2.
+Proof.
+  induction p1; induction p2; cbn in *.
+    by rewrite ccdenote_app.
+    by rewrite ccdenote_app IHp2 -orb_andb_distrib_r.
+    by rewrite ccdenote_app cdenote_bind_l -orb_andb_distrib_l.
+    specialize (IHp1 (ncons a0 p2)). cbn in *.
+      rewrite ccdenote_app cdenote_app cdenote_bind_r IHp1. solve_bool.
+Qed.
+
+Function distr_or (p : nnf_prop) : cnf_prop :=
+match p with
+    | nnf_var v => singl (singl (pos v))
+    | nnf_not v => singl (singl (neg v))
+    | nnf_and p1 p2 => distr_or p1 +++ distr_or p2
+    | nnf_or p1 p2 => nel_prod (distr_or p1) (distr_or p2)
+end.
+
+Lemma distr_or_correct :
+  forall (truth : var -> bool) (p : nnf_prop),
+    cdenote truth (distr_or p) = ndenote truth p.
+Proof.
+  intros. induction p; cbn; trivial.
+    by rewrite cdenote_app IHp1 IHp2.
+    by rewrite cdenote_nel_prod IHp1 IHp2.
+Qed.
+
+Definition cnf (f : formula) : cnf_prop :=
+  distr_or (push_not (unarrow f)).
+
+Lemma cnf_correct :
+  forall (truth : var -> bool) (f : formula),
+    cdenote truth (cnf f) = fdenote truth f.
+Proof.
+  intros. unfold cnf.
+  by rewrite distr_or_correct push_not_correct unarrow_correct.
+Qed.
+
+(* DNF translation *)
+
+Definition dnf_prop : Set := nel clause.
+
+Fixpoint dcdenote (truth : var -> bool) (dc : clause) : bool :=
+match dc with
+    | singl x => ldenote truth x
+    | ncons h t => ldenote truth h && dcdenote truth t
+end.
+
+Lemma dcdenote_app :
+  forall (truth : var -> bool) (c1 c2 : clause),
+    dcdenote truth (c1 +++ c2) = dcdenote truth c1 && dcdenote truth c2.
+Proof.
+  induction c1; cbn; intro; by rewrite // IHc1 andb_assoc.
+Qed.
+
+Fixpoint ddenote (truth : var -> bool) (p : dnf_prop) : bool :=
+match p with
+    | singl c => dcdenote truth c
+    | ncons h t => dcdenote truth h || ddenote truth t
+end.
+
+Lemma ddenote_app :
+  forall (truth : var -> bool) (p1 p2 : cnf_prop),
+    ddenote truth (p1 +++ p2) = ddenote truth p1 || ddenote truth p2.
+Proof.
+  induction p1; cbn; intro; by rewrite // IHp1 orb_assoc.
+Qed.
+
+Lemma ddenote_bind_l :
+  forall (p : cnf_prop) (truth : var -> bool) (c : clause),
+    ddenote truth (nel_bind p (fun x : nel literal => singl (x +++ c))) =
+    ddenote truth p && dcdenote truth c.
+Proof.
+  induction p; cbn; intros;
+  by rewrite dcdenote_app // IHp -andb_orb_distrib_l.
+Qed.
+
+Lemma ddenote_bind_r :
+  forall (p : cnf_prop) (truth : var -> bool) (c : clause),
+    ddenote truth (nel_bind p (fun x : nel literal => singl (c +++ x))) =
+    ddenote truth p && dcdenote truth c.
+Proof.
+  induction p; cbn; intros;
+  by rewrite dcdenote_app andb_comm // IHp -andb_orb_distrib_l.
+Qed.
+
+Ltac solve_bool' := repeat (rewrite -?orb_assoc -?andb_assoc;
+match goal with
+    | |- context [?b1 && ?b2] => destruct b1; cbn; rewrite ?andb_false_l
+    | |- context [?b1 || ?b2] => destruct b1; cbn; rewrite ?orb_true_l
+end; auto).
+
+Lemma ddenote_nel_prod :
+  forall (truth : var -> bool) (p1 p2 : cnf_prop),
+    ddenote truth (nel_prod p1 p2) = ddenote truth p1 && ddenote truth p2.
+Proof.
+  induction p1; induction p2; cbn in *.
+    by rewrite dcdenote_app.
+    by rewrite dcdenote_app IHp2 -andb_orb_distrib_r.
+    by rewrite dcdenote_app ddenote_bind_l -andb_orb_distrib_l.
+    specialize (IHp1 (ncons a0 p2)). cbn in *.
+      rewrite dcdenote_app ddenote_app ddenote_bind_r IHp1.
+      rewrite ?orb_assoc. solve_bool'.
+Qed.
+
+Fixpoint distr_and (p : nnf_prop) : dnf_prop :=
+match p with
+    | nnf_var v => singl (singl (pos v))
+    | nnf_not v => singl (singl (neg v))
+    | nnf_or p1 p2 => distr_and p1 +++ distr_and p2
+    | nnf_and p1 p2 => nel_prod (distr_and p1) (distr_and p2)
+end.
+
+Lemma distr_and_correct :
+  forall (truth : var -> bool) (p : nnf_prop),
+    ddenote truth (distr_and p) = ndenote truth p.
+Proof.
+  intros. induction p; cbn; trivial.
+    by rewrite ddenote_nel_prod IHp1 IHp2.
+    by rewrite ddenote_app IHp1 IHp2.
+Qed.
+
+Definition dnf (f : formula) : dnf_prop :=
   distr_and (push_not (unarrow f)).
 
+Lemma dnf_correct :
+  forall (truth : var -> bool) (f : formula),
+    ddenote truth (dnf f) = fdenote truth f.
+Proof.
+  intros. unfold dnf.
+  by rewrite distr_and_correct push_not_correct unarrow_correct.
+Qed.
+
+(* Tests *)
 
 Definition s := f_and (f_or (f_var 1) (f_var 2)) (f_var 3).
+Definition s' := f_or (f_and (f_var 1) (f_var 2)) (f_var 3).
 
 Compute cnf s.
+Compute cnf s'.
 Compute dnf s.
-Compute toCNF (cnf s).
-Compute toDNF (dnf s).
+Compute dnf s'.
+
+Definition empty : var -> bool := fun _ => false.
